@prefix dct: <http://purl.org/dc/terms/> .
@prefix pav: <http://purl.org/pav/> .
@prefix qudt: <http://qudt.org/schema/qudt/> .
@prefix rdf: <http://www.w3.org/1999/02/22-rdf-syntax-ns#> .
@prefix skos: <http://www.w3.org/2004/02/skos/core#> .
@prefix unit: <http://qudt.org/vocab/unit/> .
@prefix vars: <http://purl.org/m4m-dk-3/variables/> .

<http://purl.org/m4m-dk-3/variables/> a skos:Concept, skos:ConceptScheme;
  dct:creator <https://orcid.org/0000-0002-0329-0192>, <https://orcid.org/0000-0002-9381-9693>,
    <https://orcid.org/0000-0002-9823-589X>, <https://orcid.org/0000-0003-2971-3402>;
  dct:description "Quantitative and qualitative and quantitative variables describing ..."@en;
  dct:rights <https://spdx.org/licenses/CC0-1.0>;
  dct:title "ENVS variables"@en;
  pav:createdOn "2021-09-27T12:00+02:00"@en;
  pav:lastUpdatedOn "2021-09-27T13:00+02:00"@en;
  pav:version "0.1.2"@en;
  skos:hasTopConcept <http://purl.org/m4m-dk-3/variables/>, vars:AtmosphericTerms, vars:GenericTerms,
    vars:WaterTerms;
  skos:inScheme <http://purl.org/m4m-dk-3/variables/>;
  skos:topConceptOf <http://purl.org/m4m-dk-3/variables/> .

vars:AtmosphericTerms a skos:Concept;
  skos:definition "This is a parent concept containing controlled terms representing atmospheric variables."@en;
  skos:inScheme <http://purl.org/m4m-dk-3/variables/>;
  skos:narrower vars:atmospheric_pressure, vars:relative_humidity, vars:wind_direction,
    vars:wind_speed;
  skos:prefLabel "Atmospheric Terms"@en;
  skos:topConceptOf <http://purl.org/m4m-dk-3/variables/> .

vars:WaterTerms a skos:Concept;
  skos:definition "This is a parent concept containing controlled terms representing water variables."@en;
  skos:inScheme <http://purl.org/m4m-dk-3/variables/>;
  skos:narrower vars:water_temperature;
  skos:prefLabel "Water Terms"@en;
  skos:topConceptOf <http://purl.org/m4m-dk-3/variables/> .

vars:GenericTerms a skos:Concept;
  skos:definition "This is an overarching concept containing variables that are not field specific."@en;
  skos:inScheme <http://purl.org/m4m-dk-3/variables/>;
  skos:narrower vars:Latitude, vars:Longitude, vars:Propiconazole;
  skos:prefLabel "Generic Terms"@en;
  skos:topConceptOf <http://purl.org/m4m-dk-3/variables/> .

vars:wind_speed a skos:Concept;
  dct:creator <https://orcid.org/0000-0002-9381-9693>;
  qudt:unit unit:M-PER-SEC;
  skos:broader vars:AtmosphericTerms;
  skos:definition "Speed is the magnitude of velocity. Wind is defined as a two-dimensional (horizontal) air velocity vector, with no vertical component. (Vertical motion in the atmosphere has the standard name upward_air_velocity.) The wind speed is the magnitude of the wind velocity."@en;
  skos:exactMatch <https://mmisw.org/ont/cf/parameter/wind_speed>;
  skos:inScheme <http://purl.org/m4m-dk-3/variables/>;
  skos:prefLabel "wind_speed"@en .

vars:wind_direction a skos:Concept;
  qudt:unit unit:Degree;
  skos:broader vars:AtmosphericTerms;
  skos:inScheme <http://purl.org/m4m-dk-3/variables/>;
  skos:prefLabel "wind_direction"@en .

vars:Latitude a skos:Concept;
  skos:broader vars:GenericTerms;
  skos:closeMatch <https://mmisw.org/ont/cf/parameter/grid_latitude>, <https://mmisw.org/ont/cf/parameter/latitude>;
  skos:definition "Latitude is positive northward; its units of degree_north (or equivalent) indicate this explicitly. In a latitude-longitude system defined with respect to a rotated North Pole, the standard name of grid_latitude should be used instead of latitude. Grid latitude is positive in the grid-northward direction, but its units should be plain degree."@en;
  skos:inScheme <http://purl.org/m4m-dk-3/variables/>;
  skos:prefLabel "Latitude"@en .

vars:Longitude a skos:Concept;
  skos:broader vars:GenericTerms;
  skos:closeMatch <https://mmisw.org/ont/cf/parameter/grid_longitude>, <https://mmisw.org/ont/cf/parameter/longitude>;
  skos:definition "Longitude is positive eastward; its units of degree_east (or equivalent) indicate this explicitly. In a latitude-longitude system defined with respect to a rotated North Pole, the standard name of grid_longitude should be used instead of longitude. Grid longitude is positive in the grid-eastward direction, but its units should be plain degree."@en;
  skos:inScheme <http://purl.org/m4m-dk-3/variables/>;
  skos:prefLabel "Longitude"@en .

vars:relative_humidity a skos:Concept;
  skos:broader vars:AtmosphericTerms;
  skos:inScheme <http://purl.org/m4m-dk-3/variables/>;
  skos:prefLabel "relative_humidity"@en .

vars:atmospheric_pressure a skos:Concept;
  qudt:unit unit:HectoPA, unit:MilliBAR;
  skos:broader vars:AtmosphericTerms;
  skos:closeMatch <https://mmisw.org/ont/cf/parameter/air_pressure>;
  skos:definition "Air pressure is the force per unit area which would be exerted when the moving gas molecules of which the air is composed strike a theoretical surface of any orientation."@en;
  skos:inScheme <http://purl.org/m4m-dk-3/variables/>;
  skos:prefLabel "atmospheric_pressure"@en .

vars:water_temperature a skos:Concept;
  skos:broader vars:WaterTerms;
  skos:inScheme <http://purl.org/m4m-dk-3/variables/>;
  skos:prefLabel "water_temperature"@en .

vars:Propiconazole a skos:Concept;
  skos:altLabel "1-[[2-(2,4-dichlorophenyl)-4-propyl-1,3-dioxolan-2-yl]methyl]-1,2,4-triazole"@en,
    "60207-90-1"@en;
  skos:broader vars:GenericTerms;
  skos:exactMatch <https://pubchem.ncbi.nlm.nih.gov/compound/43234>;
  skos:inScheme <http://purl.org/m4m-dk-3/variables/>;
  skos:prefLabel "Propiconazole"@en .
